wip

src/sequential/SeqLift.v
@@ -34,18 +34,9 @@ Require Import MaxView.
 
 Set Implicit Arguments.
 
+
 Definition world: Type. Admitted.
 Variable world_messages_le: Messages.t -> world -> world -> Prop.
-
-Definition value_map := Loc.t -> option Const.t.
-
-Definition value_map_le (vm0 vm1: value_map): Prop :=
-  forall loc,
-    match (vm0 loc), (vm1 loc) with
-    | _, None => True
-    | Some v0, Some v1 => v0 = v1
-    | _, _ => False
-    end.
 
 
 Definition flags := Loc.t -> bool.
@@ -58,92 +49,142 @@ Definition update_flags (f: flags) (l: Loc.t) (b: bool): flags :=
   fun l' => if (Loc.eq_dec l' l) then b else f l'.
 
 
-Definition sim_local (f_src: flags) (f_tgt: flags) (b: bool) (w: world) (lc_src: Local.t) (lc_tgt: Local.t): Prop. Admitted.
+Definition sim_timemap (f_src: flags) (b: bool) (w: world) (sc_src sc_tgt: TimeMap.t): Prop. Admitted.
 
 Definition sim_memory (f_src: flags) (b: bool) (w: world) (mem_src: Memory.t) (mem_tgt: Memory.t): Prop. Admitted.
 
-Definition sim_timemap: forall (w: world) (sc_src sc_tgt: TimeMap.t), Prop. Admitted.
 
-Lemma sim_local_future f_tgt w0 w1 lc_src lc_tgt
-      (SIM: sim_local flags_bot f_tgt false w0 lc_src lc_tgt)
-      (WORLD: world_messages_le (Messages.of_memory lc_src.(Local.promises)) w0 w1)
+Definition value_map := Loc.t -> option (Const.t * Const.t).
+
+Definition value_map_le (vm0 vm1: value_map): Prop :=
+  forall loc,
+    match (vm0 loc), (vm1 loc) with
+    | _, None => True
+    | Some vs0, Some vs1 => vs0 = vs1
+    | _, _ => False
+    end.
+
+
+Definition sim_local (vm: value_map) (f_src: flags) (f_tgt: flags)
+           (b: bool) (w: world)
+           (lc_src: Local.t) (lc_tgt: Local.t)
+           (mem_src: Memory.t) (mem_tgt: Memory.t)
+           (sc_src: TimeMap.t) (sc_tgt: TimeMap.t): Prop. Admitted.
+
+
+Lemma sim_local_lower vm flags_bot f_tgt w lc_src lc_tgt0 lc_tgt1 mem_src
+      mem_tgt0 mem_tgt1 sc_src sc_tgt0 sc_tgt1
+      (SIM: sim_local vm flags_bot f_tgt false w lc_src lc_tgt0 mem_src mem_tgt0 sc_src sc_tgt0)
+      (LOCAL: lower_local lc_tgt0 lc_tgt1)
+      (MEM: lower_memory mem_tgt0 mem_tgt1)
+      (SC: TimeMap.le sc_tgt0 sc_tgt1)
   :
-    sim_local flags_bot f_tgt true w1 lc_src lc_tgt.
+    sim_local vm flags_bot f_tgt false w lc_src lc_tgt1 mem_src mem_tgt1 sc_src sc_tgt1.
 Admitted.
 
 Lemma sim_update_latest lang_src
       (st_src: lang_src.(Language.state))
-      f_tgt w lc_src lc_tgt mem_src mem_tgt sc_src
-      (LOCAL: sim_local flags_bot f_tgt true w lc_src lc_tgt)
-      (MEM: sim_memory flags_bot false w mem_src mem_tgt)
+      vm f_tgt w0 lc_src lc_tgt mem_src mem_tgt sc_src sc_tgt
+      (LOCAL: sim_local vm flags_bot f_tgt true w0 lc_src lc_tgt mem_src mem_tgt sc_src sc_tgt)
+      (MEM: sim_memory flags_bot false w0 mem_src mem_tgt)
+      (SC: sim_timemap flags_bot false w0 sc_src sc_tgt)
   :
-    exists mem_src' lc_src',
+    exists mem_src' lc_src' w1,
       (<<STEPS: rtc (@Thread.tau_step _)
                     (Thread.mk _ st_src lc_src sc_src mem_src)
                     (Thread.mk _ st_src lc_src' sc_src mem_src')>>) /\
-      (<<LOCAL: sim_local flags_bot f_tgt false w lc_src' lc_tgt>>) /\
-      (<<MEM: sim_memory flags_bot false w mem_src' mem_tgt>>).
+      (<<LOCAL: sim_local vm flags_bot f_tgt false w1 lc_src' lc_tgt mem_src' mem_tgt sc_src sc_tgt>>) /\
+      (<<MEM: sim_memory flags_bot false w1 mem_src' mem_tgt>>) /\
+      (<<SC: sim_timemap flags_bot false w1 sc_src sc_tgt>>) /\
+      (<<WORLD: world_messages_le (unchangable mem_src lc_src.(Local.promises)) w0 w1>>).
 Admitted.
 
-Lemma sim_cap f_tgt w0 lc_src lc_tgt mem_src0 mem_tgt0 mem_tgt1
-      (LOCAL: sim_local flags_bot f_tgt false w0 lc_src lc_tgt)
+Lemma sim_memory_lower f_src w mem_src mem_tgt0 mem_tgt1
+      (SIM: sim_memory f_src false w mem_src mem_tgt0)
+      (MEM: lower_memory mem_tgt0 mem_tgt1)
+  :
+    sim_memory f_src false w mem_src mem_tgt1.
+Admitted.
+
+Lemma sim_timemap_lower f_src w sc_src sc_tgt0 sc_tgt1
+      (SIM: sim_timemap f_src false w sc_src sc_tgt0)
+      (SC: TimeMap.le sc_tgt0 sc_tgt1)
+  :
+    sim_timemap f_src false w sc_src sc_tgt1.
+Admitted.
+
+
+
+
+Lemma sim_cap vm f_tgt w0 lc_src lc_tgt mem_src0 mem_tgt0 mem_tgt1 sc_src sc_tgt
+      (LOCAL: sim_local vm flags_bot f_tgt false w0 lc_src lc_tgt mem_src0 mem_tgt0 sc_src sc_tgt)
       (MEM: sim_memory flags_bot false w0 mem_src0 mem_tgt0)
+      (SC: sim_timemap flags_bot false w0 sc_src sc_tgt)
       (CAP: Memory.cap mem_tgt0 mem_tgt1)
   :
     exists tm_src mem_src1 w1,
       (<<TM: forall loc, Time.lt (Memory.max_ts loc mem_src0) (tm_src loc)>>) /\
       (<<CAP: CapFlex.cap_flex mem_src0 mem_src1 tm_src>>) /\
       (<<MEM: sim_memory flags_bot true w1 mem_src1 mem_tgt1>>) /\
-      (<<LOCAL: sim_local flags_bot f_tgt false w1 lc_src lc_tgt>>) /\
+      (<<SC: sim_timemap flags_bot true w1 sc_src sc_tgt>>) /\
+      (<<LOCAL: sim_local vm flags_bot f_tgt true w1 lc_src lc_tgt mem_src1 mem_tgt1 sc_src sc_tgt>>) /\
       (<<WORLD: world_messages_le (unchangable mem_src0 lc_src.(Local.promises)) w0 w1>>).
 Admitted.
 
-Lemma sim_local_lower flags_bot f_tgt w lc_src lc_tgt0 lc_tgt1
-      (SIM: sim_local flags_bot f_tgt false w lc_src lc_tgt0)
-      (LOCAL: lower_local lc_tgt0 lc_tgt1)
-  :
-    sim_local flags_bot f_tgt false w lc_src lc_tgt1.
-Admitted.
+Lemma sim_future vm0 f_tgt w0 lc_src lc_tgt mem_src0 mem_tgt0 sc_src0 sc_tgt0
+      (SIM: sim_local vm0 flags_bot f_tgt false w0 lc_src lc_tgt mem_src0 mem_tgt0 sc_src0 sc_tgt0)
+      (MEM0: sim_memory flags_bot false w0 mem_src0 mem_tgt0)
+      (SC0: sim_timemap flags_bot false w0 sc_src0 sc_tgt0)
 
-Lemma sim_memory_lower f_src b w mem_src mem_tgt0 mem_tgt1
-      (SIM: sim_memory f_src b w mem_src mem_tgt0)
-      (LOCAL: lower_memory mem_tgt0 mem_tgt1)
+      w1 mem_src1 mem_tgt1 sc_src1 sc_tgt1
+      (WORLD: world_messages_le (Messages.of_memory lc_src.(Local.promises)) w0 w1)
+      (MEMSRC: Memory.future mem_src0 mem_src1)
+      (MEMTGT: Memory.future mem_tgt0 mem_tgt1)
+      (SCSRC: TimeMap.le sc_src0 sc_src1)
+      (SCTGT: TimeMap.le sc_tgt0 sc_tgt1)
+      (MEM1: sim_memory flags_bot false w1 mem_src1 mem_tgt1)
+      (SC1: sim_timemap flags_bot false w1 sc_src1 sc_tgt1)
   :
-    sim_memory f_src b w mem_src mem_tgt1.
+    exists vm1,
+      (<<SIM: sim_local vm1 flags_bot f_tgt true w1 lc_src lc_tgt mem_src1 mem_tgt1 sc_src1 sc_tgt1>>) /\
+      (<<VALUES: value_map_le vm0 vm1>>)
+.
 Admitted.
 
 Lemma sim_make_promise_match lang_src
       (st_src: lang_src.(Language.state))
-      f_src f_tgt w0 lc_src lc_tgt mem_src mem_tgt sc_src
-      loc
+      vm f_src f_tgt w0 lc_src lc_tgt mem_src mem_tgt sc_src sc_tgt
+      loc v
       (FLAG: f_src loc = true)
-      (LOCAL: sim_local f_src f_tgt false w0 lc_src lc_tgt)
+      (LOCAL: sim_local vm f_src f_tgt false w0 lc_src lc_tgt mem_src mem_tgt sc_src sc_tgt)
       (MEM: sim_memory flags_bot false w0 mem_src mem_tgt)
-      (VAL: forall ts_tgt v (MAX: max_readable mem_tgt lc_tgt.(Local.promises) loc ts_tgt v),
-          exists ts_src, max_readable mem_src lc_src.(Local.promises) loc ts_src v)
+      (SC: sim_timemap flags_bot false w0 sc_src sc_tgt)
+      (VAL: vm loc = Some (v, v))
   :
     exists mem_src' lc_src' w1,
       (<<STEPS: rtc (@Thread.tau_step _)
                     (Thread.mk _ st_src lc_src sc_src mem_src)
                     (Thread.mk _ st_src lc_src' sc_src mem_src')>>) /\
-      (<<LOCAL: sim_local (update_flags f_src loc false) (update_flags f_tgt loc false) false w1 lc_src' lc_tgt>>) /\
+      (<<LOCAL: sim_local vm (update_flags f_src loc false) (update_flags f_tgt loc false) false w1 lc_src' lc_tgt mem_src' mem_tgt sc_src sc_tgt>>) /\
       (<<MEM: sim_memory f_src false w1 mem_src' mem_tgt>>) /\
       (<<WORLD: world_messages_le (unchangable mem_src lc_src.(Local.promises)) w0 w1>>).
 Admitted.
 
 Lemma sim_make_promise_not_match lang_src
       (st_src: lang_src.(Language.state))
-      f_src f_tgt w0 lc_src lc_tgt mem_src mem_tgt sc_src
-      loc
+      vm f_src f_tgt w0 lc_src lc_tgt mem_src mem_tgt sc_src sc_tgt
+      loc v_src v_tgt
       (FLAG: f_src loc = true)
-      (LOCAL: sim_local f_src f_tgt false w0 lc_src lc_tgt)
+      (LOCAL: sim_local vm f_src f_tgt false w0 lc_src lc_tgt mem_src mem_tgt sc_src sc_tgt)
       (MEM: sim_memory flags_bot false w0 mem_src mem_tgt)
+      (SC: sim_timemap flags_bot false w0 sc_src sc_tgt)
+      (VAL: vm loc = Some (v_src, v_tgt))
   :
     exists mem_src' lc_src' w1,
       (<<STEPS: rtc (@Thread.tau_step _)
                     (Thread.mk _ st_src lc_src sc_src mem_src)
                     (Thread.mk _ st_src lc_src' sc_src mem_src')>>) /\
-      (<<LOCAL: sim_local (update_flags f_src loc false) (update_flags f_tgt loc true) false w1 lc_src' lc_tgt>>) /\
+      (<<LOCAL: sim_local vm (update_flags f_src loc false) (update_flags f_tgt loc true) false w1 lc_src' lc_tgt mem_src' mem_tgt sc_src sc_tgt>>) /\
       (<<MEM: sim_memory f_src false w1 mem_src' mem_tgt>>) /\
       (<<WORLD: world_messages_le (unchangable mem_src lc_src.(Local.promises)) w0 w1>>).
 Admitted.
